tuning a bit in ConnInvariant; removing an assume in TLS.fst

src/tls/ConnInvariant.fst
@@ -185,7 +185,13 @@ val ms_derive_is_ok: h0:HyperHeap.t -> h1:HyperHeap.t -> i:AE.id -> w:MS.writer 
 		         HH.contains_ref (MR.as_rref (StreamAE.ilog (StreamAE.State.log w))) h1 /\  //the log exists in h1
 			 MR.m_sel h1 (AE.ilog (StreamAE.State.log w)) = Seq.createEmpty)))))       //and w is as yet unused
 	 (ensures (mc_inv h1))
-#reset-options "--initial_fuel 0 --max_fuel 0 --initial_ifuel 1 --max_ifuel 1"
+val invertOption : a:Type -> Lemma 
+  (requires True)
+  (ensures (forall (x:option a). is_None x \/ is_Some x))
+  [SMTPatT (option a)]
+let invertOption a = ()  
+	 
+#reset-options "--initial_fuel 0 --max_fuel 0 --initial_ifuel 0 --max_ifuel 0"	 
 let ms_derive_is_ok h0 h1 i w = 
   let aux :  j:id -> Lemma (let new_ms = MR.m_sel h1 MS.ms_tab in
   			  let new_conn = MR.m_sel h1 conn_tab in
@@ -343,7 +349,6 @@ val mutate_registered_writer_ok : h0:HH.t -> h1:HH.t -> i:AE.id{authId i} -> w:M
 	       MM.sel (MR.m_sel h0 conn_tab) (I.nonce_of_id i) = Some c /\ //the connection is logged in the conn_table
 	       HH.contains_ref (MR.as_rref (StreamAE.ilog (StreamAE.State.log w))) h1)) //We say that we changed the w.region; but that doesn't necessarily mean that its log remains
     (ensures (mc_inv h1))
-#reset-options "--initial_fuel 0 --max_fuel 0 --initial_ifuel 0 --max_ifuel 0"
 let mutate_registered_writer_ok h0 h1 i w c = (* () *)
 (* a slightly more detailed proof: *)
     let new_ms = MR.m_sel h1 MS.ms_tab in
@@ -382,7 +387,7 @@ val add_connection_ok: h0:HH.t -> h1:HH.t -> i:id -> c:i_conn i -> Lemma
 	      MM.sel old_conn nonce = None /\        //c wasn't in the table initially
 	      new_conn = MM.upd old_conn nonce c))) //and the conn_tab changed just by adding c
   (ensures (mc_inv h1))
-#reset-options "--initial_fuel 0 --max_fuel 0 --initial_ifuel 1 --max_ifuel 1"
+#reset-options "--initial_fuel 0 --max_fuel 0 --initial_ifuel 1 --max_ifuel 1" //NS: this one seems to require an inversion somewhere, but not sure exactly where
 let add_connection_ok h0 h1 i c =
     cut (HH.contains_ref (MR.as_rref conn_tab) h1);
     let old_ms = MR.m_sel h0 MS.ms_tab in
@@ -390,10 +395,14 @@ let add_connection_ok h0 h1 i c =
     let old_conn = MR.m_sel h0 conn_tab in
     let new_conn = MR.m_sel h1 conn_tab in
     let hs_region_exists : n:random -> Lemma
-    	(is_Some (MM.sel new_conn n) ==> conn_hs_region_exists (Some.v (MM.sel new_conn n)) h1) =
+    	(match MM.sel new_conn n with
+	 | None -> True
+	 | Some v -> conn_hs_region_exists v h1) =
       fun n -> match MM.sel new_conn n with
     	    | None -> ()
     	    | Some c' -> if c = c' then ()
-    		        else cut (c' = Some.v (MM.sel old_conn n)) in
+    		        else match MM.sel old_conn n with
+			     | None -> ()
+			     | Some c'' -> cut (c' = c'') in// Some.v (MM.sel old_conn n)) in
     qintro hs_region_exists;
     cut (handshake_regions_exists new_conn h1)
